1. Show that the Lagrangian is $L = \frac{1}{2}m\left(\dot{r}^{2} + r^{2}\dot{\theta}^{2}\right) + \frac{GmM_{T}}{r}$.

First note that we have $v = \dot{r}\hat{e}_{r} + r\dot{\theta}\hat{e}_{\theta}$, so then,
$$\begin{align*}
v^{2} &= v\cdot v\\
&= (\dot{r}\hat{e}_{r} + r\dot{\theta}\hat{e}_{\theta})\cdot(\dot{r}\hat{e}_{r} + r\dot{\theta}\hat{e}_{\theta})\\
&= \dot{r}^{2}(\hat{e}_{r}\cdot\hat{e}_{r}) + r^{2}\dot{\theta}^{2}(\hat{e}_\theta\cdot\hat{e}_{\theta})+ (...)(\hat{e}_{r}\cdot\hat{e}_{\theta})\\
&= \dot{r}^{2} + r^{2}\dot{\theta}^{2}.
\end{align*}$$
The kinetic energy is $K=\frac{1}{2}mv^{2} = \frac{1}{2}m(\dot{r}^{2} + r^{2}\dot{\theta}^{2})$, and the potential energy is given by $V = \frac{-GmM_{T}}{r}$, so the Lagrangian is,
$$\begin{align*}
L &= K-V\\
&= \frac{1}{2}m(\dot{r}^{2}+r^{2}\dot{\theta}^{2}) + \frac{GmM_{T}}{r}.
\end{align*}$$

2. 